mppa_k1c/Asmblockgenproof0.v
@@ -1,0 +1,95 @@
+Require Import Coqlib.
+Require Intv.
+Require Import AST.
+Require Import Errors.
+Require Import Integers.
+Require Import Floats.
+Require Import Values.
+Require Import Memory.
+Require Import Globalenvs.
+Require Import Events.
+Require Import Smallstep.
+Require Import Locations.
+Require Import Machblock.
+Require Import Asmblock.
+Require Import Asmblockgen.
+
+Module MB:=Machblock.
+Module AB:=Asmblock.
+
+(* inspired from Mach *)
+
+Lemma find_label_tail:
+  forall lbl c c', MB.find_label lbl c = Some c' -> is_tail c' c.
+Proof.
+  induction c; simpl; intros. discriminate.
+  destruct (MB.is_label lbl a). inv H. auto with coqlib. eauto with coqlib.
+Qed.
+
+(* inspired from Asmgenproof0 *)
+
+(* ... skip ... *)
+
+(** The ``code tail'' of an instruction list [c] is the list of instructions
+  starting at PC [pos]. *)
+
+Inductive code_tail: Z -> bblocks -> bblocks -> Prop :=
+  | code_tail_0: forall c,
+      code_tail 0 c c
+  | code_tail_S: forall pos bi c1 c2,
+      code_tail pos c1 c2 ->
+      code_tail (pos + (size bi)) (bi :: c1) c2.
+
+Lemma code_tail_pos:
+  forall pos c1 c2, code_tail pos c1 c2 -> pos >= 0.
+Proof.
+  induction 1. omega. generalize (size_positive bi); intros; omega.
+Qed.
+
+Lemma find_bblock_tail:
+  forall c1 bi c2 pos,
+  code_tail pos c1 (bi :: c2) ->
+  find_bblock pos c1 = Some bi.
+Proof.
+  induction c1; simpl; intros.
+  inversion H.  
+  destruct (zlt pos 0). generalize (code_tail_pos _ _ _ H); intro; omega.
+  destruct (zeq pos 0). subst pos.
+  inv H. auto. generalize (size_positive a) (code_tail_pos _ _ _ H4). intro; omega.
+  inv H. congruence. replace (pos0 + size a - size a) with pos0 by omega.
+  eauto.
+Qed.
+
+(* ... skip ... *)
+
+
+(** Predictor for return addresses in generated Asm code.
+
+  The [return_address_offset] predicate defined here is used in the
+  semantics for Mach to determine the return addresses that are
+  stored in activation records. *)
+
+(** Consider a Mach function [f] and a sequence [c] of Mach instructions
+  representing the Mach code that remains to be executed after a
+  function call returns.  The predicate [return_address_offset f c ofs]
+  holds if [ofs] is the integer offset of the PPC instruction
+  following the call in the Asm code obtained by translating the
+  code of [f]. Graphically:
+<<
+     Mach function f    |--------- Mcall ---------|
+         Mach code c    |                |--------|
+                        |                 \        \
+                        |                  \        \
+                        |                   \        \
+     Asm code           |                    |--------|
+     Asm function       |------------- Pcall ---------|
+
+                        <-------- ofs ------->
+>>
+*)
+
+Definition return_address_offset (f: MB.function) (c: MB.code) (ofs: ptrofs) : Prop :=
+  forall tf  tc,
+  transf_function f = OK tf ->
+  transl_blocks f c = OK tc ->
+  code_tail (Ptrofs.unsigned ofs) (fn_blocks tf) tc.
